\documentclass[12pt]{article}

\usepackage{amsmath}
\usepackage{eulervm}

\begin{document}

$$\sum_i P(\mathcal{H}_i\,|\,\mathcal{C})=1$$
$$P(\mathcal{H}_A,\mathcal{H}_B\,|\,\mathcal{C})=P(\mathcal{H}_A\,|\,\mathcal{H}_B,\mathcal{C})\times P(\mathcal{H}_B\,|\,\mathcal{C})$$

$$P(L\,|\,\mathcal{C})=0,76$$
$$P(S\,|\,\mathcal{C})=0,24$$
$$P(S\,|\,\mathcal{C})=1-P(L\,|\,\mathcal{C})$$

$$P(N\,|\,\mathcal{C})=0,63$$
$$P(L\,|\,N,\mathcal{C})=0,81$$
$$P(L,\bar{N}\,|\,\mathcal{C})\leq \left[1-P(L\,|\,N,\mathcal{C})\right]\times P(\bar{N}\,|\,\mathcal{C})$$
$$P(L,\bar{N}\,|\,\mathcal{C})\leq 0,07$$

\newpage

$$P(\mathcal{H}\,|\,\mathcal{D},\mathcal{C})=\frac{P(\mathcal{D}\,|\,\mathcal{H},\mathcal{C})\times P(\mathcal{H}\,|\,\mathcal{C})}{P(\mathcal{D\,|\,\mathcal{C}})}$$

$$P(\mathcal{H}\,|\,\mathcal{D},\mathcal{C})\propto P(\mathcal{D}\,|\,\mathcal{H},\mathcal{C})\times P(\mathcal{H}\,|\,\mathcal{C})$$

\newpage

$$\mathcal{L}(m,b\,|\,\{y\},\{x\},\{\sigma_y\})\propto\prod_i\exp{\left[-\frac{(\mu(m,b;x_i)-y_i)^2}{2{\sigma_y}_i^2}\right]}$$

\begin{align*}\mathcal{L}(m\,|\,\{y\},\{x\},\{\sigma_y\}) &= \int_b \mathcal{L}(m,b\,|\,\{y\},\{x\},\{\sigma_y\}) \\\mathcal{L}(b\,|\,\{y\},\{x\},\{\sigma_y\}) &= \int_m \mathcal{L}(m,b\,|\,\{y\},\{x\},\{\sigma_y\})\end{align*}

$$P(m,b\,|\,\{y\},\{x\},\{\sigma_y\})\propto \mathcal{L}(m,b\,|\,\{y\},\{x\},\{\sigma_y\})\times P(m,b\,|\,\{x\},\{\sigma_y\})$$

\newpage

$$\mathcal{L}(\mathcal{H}\,|\,\mathcal{D},\mathcal{C}),\,P(\mathcal{H}\,|\,\mathcal{C})\,\longrightarrow\,$$

$$L(P,P';\mathcal{H})\equiv\int_\mathcal{H}P(\mathcal{H}\,|\,\mathcal{C})\times\log{1/P(\mathcal{H}\,|\,\mathcal{C})}-\sum_{i=0}\lambda_i\,g_i(P,P';\mathcal{H})$$

$$\max{H}:\,\frac{\partial L}{\partial P}-\frac{d}{d\mathcal{H}}\frac{\partial L}{\partial P'}=0$$

\end{document}
